rt refine: prove refillNew_invs' and refillUpdate_invs'
In order to prove these lemmas, a conjunct is added to
valid_sched_context', roughly stating that the length
of the refill buffer is as great as possible, given the
size of the scheduling context

Signed-off-by: Michael McInerney <m.mcinerney@unsw.edu.au>

proof/refine/ARM/Invariants_H.thy
@@ -670,7 +670,8 @@ definition valid_sched_context' :: "sched_context \<Rightarrow> kernel_state \<R
      \<and> scRefillMax sc \<le> length (scRefills sc)
      \<and> (0 < scRefillMax sc \<longrightarrow> scRefillHead sc < scRefillMax sc
                                \<and> scRefillCount sc \<le> scRefillMax sc
-                               \<and> 0 < scRefillCount sc)"
+                               \<and> 0 < scRefillCount sc)
+     \<and> length (scRefills sc) = refillAbsoluteMax' (scBitsFromRefillLength' (length (scRefills sc)))"
 
 definition valid_reply' :: "reply \<Rightarrow> kernel_state \<Rightarrow> bool" where
   "valid_reply' reply s \<equiv>
